Finish Case case of pure_to_thunkProof

compiler/backend/passes/proofs/pure_to_thunkProofScript.sml
@@ -8,14 +8,17 @@ open stringTheory optionTheory sumTheory pairTheory listTheory alistTheory
      pure_semanticsTheory thunk_semanticsTheory pure_evalTheory
      thunkLang_primitivesTheory pure_exp_lemmasTheory pure_miscTheory
      pure_to_thunk_1ProofTheory pure_cexpTheory pureLangTheory
-     thunk_case_liftProofTheory
-     thunk_case_d2bProofTheory
+     thunk_case_liftProofTheory arithmeticTheory combinTheory
+     thunk_case_projProofTheory
+     thunk_let_forceProofTheory
+     thunk_cexpTheory
      expof_caseProofTheory;
 
 val _ = new_theory "pure_to_thunkProof";
 
-val _ = set_grammar_ancestry ["pure_to_thunk_1Proof", "pure_cexp",
-                              "thunkLang", "pureLang", "expof_caseProof"];
+val _ = set_grammar_ancestry
+          ["pure_to_thunk_1Proof", "pure_cexp",
+           "thunkLang", "thunk_cexp", "pureLang", "expof_caseProof"];
 
 (*
   cexp = Var 'a vname                         (* variable                 *)
@@ -59,51 +62,53 @@ Definition rows_of_def:
 End
 
 (*
-       | Prim 'a cop (cexp list)                 (* primitive operations     *)
+  TODO: Prim 'a cop (cexp list)                 (* primitive operations     *)
 *)
 
 Inductive exp_rel:
 [~Var:]
   (∀(n:mlstring).
      exp_rel (pure_cexp$Var i n)
-             (thunkLang$Force (Var (explode n)))) ∧
+             (thunk_cexp$Force (Var n))) ∧
 [~Lam:]
   (∀(s:mlstring list) x y.
      exp_rel x y ⇒
-       exp_rel (pure_cexp$Lam i s x) (Lams (MAP explode s) y)) ∧
+       exp_rel (pure_cexp$Lam i s x) (Lam s y)) ∧
 [~Let:]
-  (∀s x y.
+  (∀s x y x1 y1.
      exp_rel x x1 ∧ exp_rel y y1 ⇒
-       exp_rel (Let i s x y) (Let (SOME (explode s)) (Delay x1) y1)) ∧
+       exp_rel (Let i s x y) (Let (SOME s) (Delay x1) y1)) ∧
 [~Letrec:]
   (∀i xs xs1 y y1.
-     LIST_REL (λ(n,x) (m,x1). explode n = m ∧
+     LIST_REL (λ(n,x) (m,x1). n = m ∧
                               ∃y. exp_rel x y ∧ x1 = Delay y) xs xs1 ∧ exp_rel y y1 ⇒
        exp_rel (Letrec i xs y) (Letrec xs1 y1)) ∧
 [~App:]
   (∀f g xs ys.
      exp_rel f g ∧
      LIST_REL exp_rel xs ys ⇒
-       exp_rel (App i f xs) (Apps g (MAP Delay ys))) ∧
+       exp_rel (App i f xs) (App g (MAP Delay ys))) ∧
 [~Case:]
   (∀i x v xs ys fresh.
      ~MEM v (FLAT (MAP (FST ∘ SND) xs)) ∧ xs ≠ [] ∧
      LIST_REL (λ(x1,x2,x3) (y1,y2,y3).
-       explode x1 = y1 ∧ MAP explode x2 = y2 ∧
-       exp_rel x3 y3 ∧ fresh ∉ freevars (exp_of' x3)) xs ys ∧
-     (∀x. eopt = SOME x ⇒ fresh ∉ freevars (exp_of' x)) ∧
-     exp_rel x a_exp ∧ fresh ≠ explode v ∧
+       x1 = y1 ∧ x2 = y2 ∧ ~MEM fresh x2 ∧
+       exp_rel x3 y3 ∧ explode fresh ∉ freevars (exp_of' x3)) xs ys ∧
+     (∀x. eopt = SOME x ⇒ explode fresh ∉ freevars (exp_of' x)) ∧
+     exp_rel x a_exp ∧ fresh ≠ v ∧
      OPTREL exp_rel eopt yopt ⇒
        exp_rel (Case i x v xs eopt)
-         (Let (SOME fresh) a_exp $
-          Let (SOME (explode v)) (Box (Var fresh)) $
-            rows_of (explode v) yopt ys))
+               (Let (SOME v) (Delay a_exp) $
+                Let (SOME fresh) (Force (Var v)) $
+                  Case fresh ys yopt))
 End
 
 Overload to_thunk = “pure_to_thunk_1Proof$compile_rel”
 Overload lift_rel = “thunk_case_liftProof$compile_rel”
-Overload d2b_rel = “thunk_case_d2bProof$exp_rel”
+Overload force_rel = “thunk_let_forceProof$exp_rel”
+Overload proj_rel = “thunk_case_projProof$compile_rel”
 
+(*
 Theorem LIST_REL_combined_IMP:
   ∀xs ys.
     LIST_REL (λx y.
@@ -279,23 +284,240 @@ Proof
   \\ irule to_thunk_lets_for \\ fs []
 QED
 
+*)
+
+
+(* TODO: move to thunkLang *)
+
+Definition lets_for_def:
+  lets_for l cn v [] b = (b:thunkLang$exp) ∧
+  lets_for l cn v ((n,w)::ws) b =
+    Seq (If (IsEq cn l T (Var v)) Unit Fail) $
+      Let (SOME w) (Proj cn n (Var v)) $
+        lets_for l cn v ws b
+End
+
+Definition rows_of_def:
+  rows_of v k [] = (k:thunkLang$exp) ∧
+  rows_of v k ((cn,vs,b)::rest) =
+    If (IsEq cn (LENGTH vs) T (Var v))
+      (lets_for (LENGTH vs) cn v (MAPi (λi v. (i,v)) vs) b) (rows_of v k rest)
+End
+
+Definition op_of_def[simp]:
+  op_of (Cons m) = Cons (explode m) ∧
+  op_of (AtomOp a) = AtomOp a
+End
+
+Definition exp_of_def[simp]:
+  exp_of (Var n)         = Var (explode n):thunkLang$exp ∧
+  exp_of (Prim p xs)     = Prim (op_of p) (MAP exp_of xs) ∧
+  exp_of (Let w x y)     = Let (OPTION_MAP explode w) (exp_of x) (exp_of y) ∧
+  exp_of (App f xs)      = Apps (exp_of f) (MAP exp_of xs) ∧
+  exp_of (Lam vs x)      = Lams (MAP explode vs) (exp_of x) ∧
+  exp_of (Letrec rs x)   = Letrec (MAP (λ(n,x). (explode n,exp_of x)) rs) (exp_of x) ∧
+  exp_of (Case v rs opt) =
+      rows_of
+        (explode v)
+        (case opt of NONE => Fail | SOME e => exp_of e)
+        (MAP (λ(c,vs,x). (explode c,MAP explode vs,exp_of x)) rs) ∧
+  exp_of (Force x)       = Force (exp_of x) ∧
+  exp_of (Delay x)       = Delay (exp_of x) ∧
+  exp_of (Box x)         = Box (exp_of x)
+Termination
+  WF_REL_TAC ‘measure cexp_size’ >> rw [cexp_size_eq]
+End
+
+(* --- *)
+
+Overload VV[local] = “thunk_let_forceProof$Var”
+
 val to_thunk_freevars = pure_to_thunk_1ProofTheory.compile_rel_freevars;
+
+Theorem lets_for_lemma[local]:
+  ∀vs k.
+    to_thunk (exp_of' h2) y1 ∧
+    lift_rel y1 y2 ∧
+    force_rel NONE y2 y3 ∧
+    proj_rel y3 (exp_of yy2) ∧
+    ~MEM fresh vs ∧ ~MEM h vs ∧ fresh ≠ h ∧
+    fresh ∉ freevars (exp_of' h2) ⇒
+    ∃x1 x2 x3.
+      to_thunk
+        (lets_for' (k + LENGTH vs) cn h
+          (MAPi (λx v. (x+k,v)) vs) (exp_of' h2)) x1 ∧
+      lift_rel x1 x2 ∧ fresh ∉ freevars x1 ∧
+      force_rel (SOME (VV h,fresh)) x2 x3 ∧
+      proj_rel x3
+        (lets_for (k + LENGTH vs) cn fresh
+          (MAPi (λx v. (x+k,v)) vs) (exp_of yy2))
+Proof
+  Induct
+  \\ fs [lets_for_def,lets_for'_def]
+  >-
+   (rw [] \\ imp_res_tac to_thunk_freevars
+    \\ rpt $ first_x_assum $ irule_at Any \\ fs []
+    \\ irule thunk_let_forceProofTheory.exp_rel_NONE_IMP_SOME \\ fs [])
+  \\ rw [] \\ gvs []
+  \\ simp [Once pure_to_thunk_1ProofTheory.compile_rel_cases, PULL_EXISTS]
+  \\ simp [Once pure_to_thunk_1ProofTheory.compile_rel_cases, PULL_EXISTS]
+  \\ simp [Once pure_to_thunk_1ProofTheory.compile_rel_cases, PULL_EXISTS]
+  \\ simp [Once pure_to_thunk_1ProofTheory.compile_rel_cases, PULL_EXISTS]
+  \\ simp [Once pure_to_thunk_1ProofTheory.compile_rel_cases, PULL_EXISTS]
+  \\ simp [Once pure_to_thunk_1ProofTheory.compile_rel_cases, PULL_EXISTS]
+  \\ irule_at Any pure_to_thunk_1ProofTheory.compile_rel_Let
+  \\ irule_at Any pure_to_thunk_1ProofTheory.compile_rel_Proj \\ fs [PULL_EXISTS]
+  \\ irule_at Any pure_to_thunk_1ProofTheory.compile_rel_Var
+  \\ irule_at Any thunk_case_projProofTheory.compile_rel_Proj \\ fs []
+  \\ fs [o_DEF,freevars_def]
+  \\ last_x_assum $ qspec_then ‘SUC k’ mp_tac
+  \\ fs [ADD_CLAUSES] \\ rw []
+  \\ rpt $ first_x_assum $ irule_at Any
+  \\ irule_at Any thunk_case_liftProofTheory.compile_rel_Let
+  \\ irule_at Any thunk_case_liftProofTheory.compile_rel_If \\ fs []
+  \\ irule_at Any thunk_case_liftProofTheory.compile_rel_Prim \\ fs [PULL_EXISTS]
+  \\ irule_at Any thunk_case_liftProofTheory.compile_rel_Prim \\ fs [PULL_EXISTS]
+  \\ irule_at Any thunk_case_liftProofTheory.compile_rel_Prim \\ fs [PULL_EXISTS]
+  \\ irule_at Any thunk_case_liftProofTheory.compile_rel_Force
+  \\ irule_at Any thunk_case_liftProofTheory.compile_rel_Var
+  \\ irule_at Any thunk_case_liftProofTheory.compile_rel_Let
+  \\ irule_at Any thunk_case_liftProofTheory.compile_rel_Delay
+  \\ irule_at Any thunk_case_liftProofTheory.compile_rel_Force
+  \\ irule_at Any thunk_case_liftProofTheory.compile_rel_Prim \\ fs [PULL_EXISTS]
+  \\ irule_at Any thunk_case_liftProofTheory.compile_rel_Force
+  \\ irule_at Any thunk_case_liftProofTheory.compile_rel_Var
+  \\ rpt $ first_x_assum $ irule_at Any
+  \\ irule_at Any thunk_let_forceProofTheory.exp_rel_Let
+  \\ fs [name_clash_def]
+  \\ irule_at Any thunk_let_forceProofTheory.exp_rel_Let
+  \\ fs [name_clash_def]
+  \\ rpt $ simp [Once thunk_let_forceProofTheory.exp_rel_cases]
+QED
+
+Triviality MEM_EQ_MEM_MAP_explode:
+  ∀h1 f. MEM f h1 ⇔ MEM (explode f) (MAP explode h1)
+Proof
+  Induct \\ fs []
+QED
 
 Theorem exp_rel_imp_combined:
   ∀x y.
     exp_rel x y ∧ cexp_wf x ⇒
-    ∃y1 y2.
+    ∃y1 y2 y3.
       to_thunk (exp_of' x) y1 ∧
       lift_rel y1 y2 ∧
-      d2b_rel y2 y
+      force_rel NONE y2 y3 ∧
+      proj_rel y3 (exp_of y)
 Proof
+
   Induct_on ‘exp_rel’ \\ rw [exp_of'_def,cexp_wf_def] \\ fs []
   >~ [‘Var n’] >-
    (simp [Once pure_to_thunk_1ProofTheory.compile_rel_cases]
     \\ irule_at Any thunk_case_liftProofTheory.compile_rel_Force
-    \\ irule_at Any thunk_case_d2bProofTheory.exp_rel_Force
-    \\ irule_at Any thunk_case_d2bProofTheory.exp_rel_Var
-    \\ irule_at Any thunk_case_liftProofTheory.compile_rel_Var)
+    \\ irule_at Any thunk_case_liftProofTheory.compile_rel_Var
+    \\ irule_at Any thunk_let_forceProofTheory.exp_rel_Force
+    \\ irule_at Any thunk_let_forceProofTheory.exp_rel_Var
+    \\ irule_at Any thunk_case_projProofTheory.compile_rel_Force
+    \\ irule_at Any thunk_case_projProofTheory.compile_rel_Var)
+  >~ [‘rows_of'’] >-
+   (irule_at Any thunk_case_projProofTheory.compile_rel_Let_SOME
+    \\ irule_at Any thunk_let_forceProofTheory.exp_rel_Let
+    \\ irule_at Any thunk_case_liftProofTheory.compile_rel_Let
+    \\ fs [name_clash_def]
+    \\ simp [Once pure_to_thunk_1ProofTheory.compile_rel_cases,PULL_EXISTS]
+    \\ irule_at Any thunk_case_liftProofTheory.compile_rel_Delay
+    \\ irule_at Any thunk_let_forceProofTheory.exp_rel_Delay
+    \\ irule_at Any thunk_case_projProofTheory.compile_rel_Delay
+    \\ qpat_x_assum ‘proj_rel y3 (exp_of y)’ $ irule_at Any
+    \\ qpat_x_assum ‘force_rel NONE y2 y3’ $ irule_at Any
+    \\ qpat_x_assum ‘lift_rel y1 y2’ $ irule_at Any
+    \\ qpat_x_assum ‘to_thunk (exp_of' x) y1’ $ irule_at Any
+    \\ Cases_on ‘xs’ \\ fs []
+    \\ PairCases_on ‘h’ \\ fs []
+    \\ rename [‘_ = yy :: _’]
+    \\ PairCases_on ‘yy’ \\ gvs [rows_of'_def]
+    \\ simp [Once pure_to_thunk_1ProofTheory.compile_rel_cases,PULL_EXISTS]
+    \\ simp [Once pure_to_thunk_1ProofTheory.compile_rel_cases,PULL_EXISTS]
+    \\ simp [Once pure_to_thunk_1ProofTheory.compile_rel_cases,PULL_EXISTS]
+    \\ irule_at Any thunk_case_liftProofTheory.compile_rel_Lift
+    \\ irule_at Any thunk_case_liftProofTheory.compile_rel_Force
+    \\ irule_at Any thunk_case_liftProofTheory.compile_rel_Var
+    \\ fs [freevars_def]
+    \\ irule_at Any thunk_case_projProofTheory.compile_rel_Let_SOME
+    \\ irule_at Any thunk_case_projProofTheory.compile_rel_Force
+    \\ irule_at Any thunk_case_projProofTheory.compile_rel_Var
+    \\ irule_at Any thunk_let_forceProofTheory.exp_rel_Let_Force_Var
+    \\ fs []
+    \\ irule_at Any thunk_let_forceProofTheory.exp_rel_If \\ fs []
+    \\ irule_at Any thunk_let_forceProofTheory.exp_rel_Prim \\ fs [PULL_EXISTS]
+    \\ irule_at Any thunk_let_forceProofTheory.exp_rel_Force_Var
+    \\ fs [rows_of_def]
+    \\ irule_at Any thunk_case_projProofTheory.compile_rel_If \\ fs []
+    \\ irule_at Any thunk_case_projProofTheory.compile_rel_Prim \\ fs []
+    \\ irule_at Any thunk_case_projProofTheory.compile_rel_Var \\ fs []
+    \\ drule lets_for_lemma
+    \\ rpt $ disch_then drule
+    \\ ‘¬MEM (explode fresh) (MAP explode h1)’ by fs [MEM_EQ_MEM_MAP_explode]
+    \\ disch_then drule
+    \\ ‘¬MEM (explode v) (MAP explode h1)’ by fs [MEM_EQ_MEM_MAP_explode]
+    \\ disch_then drule
+    \\ disch_then $ qspecl_then [‘explode h0’,‘0’] strip_assume_tac
+    \\ gvs []
+    \\ rpt $ pop_assum $ irule_at Any
+    \\ rename [‘LIST_REL _ ys1 ys2’]
+    \\ qpat_x_assum ‘LIST_REL _ _ _’ mp_tac
+    \\ qpat_x_assum ‘EVERY _ _’ mp_tac
+    \\ qpat_x_assum ‘¬MEM v (FLAT (MAP (FST ∘ SND) ys1))’ mp_tac
+    \\ qid_spec_tac ‘ys2’
+    \\ qid_spec_tac ‘ys1’
+    \\ Induct \\ fs [PULL_EXISTS]
+    >-
+     (fs [rows_of_def,rows_of'_def]
+      \\ Cases_on ‘yopt’ \\ fs []
+      >-
+       (irule_at Any thunk_case_projProofTheory.compile_rel_Prim \\ fs []
+        \\ irule_at Any thunk_let_forceProofTheory.exp_rel_Prim \\ fs []
+        \\ irule_at Any thunk_case_liftProofTheory.compile_rel_Prim \\ fs []
+        \\ Cases_on ‘eopt’ \\ fs []
+        \\ simp [Once pure_to_thunk_1ProofTheory.compile_rel_cases, freevars_def])
+      \\ Cases_on ‘eopt’ \\ fs []
+      \\ rpt $ first_assum $ irule_at Any
+      \\ irule_at Any thunk_let_forceProofTheory.exp_rel_NONE_IMP_SOME
+      \\ fs [] \\ imp_res_tac to_thunk_freevars \\ fs [])
+    \\ fs [FORALL_PROD]
+    \\ rw [] \\ gvs []
+    \\ first_x_assum dxrule
+    \\ strip_tac
+    \\ fs [rows_of_def,rows_of'_def]
+    \\ simp [Once pure_to_thunk_1ProofTheory.compile_rel_cases,PULL_EXISTS]
+    \\ simp [Once pure_to_thunk_1ProofTheory.compile_rel_cases,PULL_EXISTS]
+    \\ simp [Once pure_to_thunk_1ProofTheory.compile_rel_cases,PULL_EXISTS]
+    \\ fs [freevars_def]
+    \\ qpat_x_assum ‘to_thunk _ _’ $ irule_at Any
+    \\ irule_at Any thunk_case_liftProofTheory.compile_rel_If \\ fs [PULL_EXISTS]
+    \\ irule_at Any thunk_case_liftProofTheory.compile_rel_Prim \\ fs [PULL_EXISTS]
+    \\ irule_at Any thunk_case_liftProofTheory.compile_rel_Force
+    \\ irule_at Any thunk_case_liftProofTheory.compile_rel_Var
+    \\ irule_at Any thunk_case_projProofTheory.compile_rel_If \\ fs [PULL_EXISTS]
+    \\ irule_at Any thunk_case_projProofTheory.compile_rel_Prim \\ fs [PULL_EXISTS]
+    \\ irule_at Any thunk_case_projProofTheory.compile_rel_Var
+    \\ simp [Once thunk_let_forceProofTheory.exp_rel_cases]
+    \\ simp [Once thunk_let_forceProofTheory.exp_rel_cases]
+    \\ simp [Once thunk_let_forceProofTheory.exp_rel_cases]
+    \\ drule lets_for_lemma
+    \\ ntac 3 $ disch_then drule
+    \\ disch_then $ drule_at $ Pos last
+    \\ rename [‘lets_for' (LENGTH cs) (explode cn)’]
+    \\ disch_then $ qspecl_then [‘explode v’,
+            ‘explode cn’,‘MAP explode cs’,‘0’] mp_tac
+    \\ impl_tac >- fs [GSYM MEM_EQ_MEM_MAP_explode]
+    \\ fs [] \\ strip_tac
+    \\ rpt $ pop_assum $ irule_at Any
+    \\ first_assum $ irule_at Any
+    \\ first_assum $ irule_at Any)
+
+  \\ cheat
+(*
   >~ [‘Lams s’] >-
    (qid_spec_tac ‘s’ \\ Induct
     \\ fs [Lams_def,pure_expTheory.Lams_def]
@@ -406,12 +628,18 @@ Proof
   \\ Cases_on ‘eopt’ \\ gvs [OPTREL_SIMP,PULL_EXISTS]
   \\ rpt $ first_assum $ irule_at Any
   \\ imp_res_tac to_thunk_freevars \\ fs []
+  *)
 QED
 
 (*
 
-TODO:
- - make thunk_case_inl usable
+new order:
+
+thunk_case_lift:    If IsEq --> Let If IsEq       -- has cheat
+thunk_let_force:    Let (SOME w) (Force (Var v)) enables rewrite Force (Var v) --> Var w
+thunk_case_proj:    Let (SOME w) (Delay (Force (Proj s i (Var v)))) x --> Let (SOME w) (Proj s i (Var v)) y -- has cheat
+
+old order:
 
 thunk_case_lift:    If IsEq --> Let If IsEq       -- has cheat
 thunk_case_d2b:     Let Delay Force --> Let Box
